Reached Clight

cfrontend/Cexecimpl_old.v
@@ -1,5 +1,5 @@
-Require Cexec.
-Require Memory.
+Require Cexec_old.
+Require Memimpl.
 
 (** * Instantiate Cexec with a memory model and external functions.
 
@@ -11,6 +11,11 @@ Require Memory.
    driver/Interp.ml.
  *)
 
+(** ** Memory model. *)
+
+Local Existing Instance Memimpl.Mem.memory_model_ops.
+Local Existing Instance Memimpl.Mem.memory_model_prf.
+
 (** ** External function semantics.
 
     In Interp.ml, do_external_function is used for all three of
@@ -19,8 +24,8 @@ Require Memory.
 
 Parameter do_external_function:
   String.string -> AST.signature -> Globalenvs.Senv.t ->
-  Determinism.world -> list Values.val -> Memory.mem ->
-  option (Determinism.world * Events.trace * Values.val * Memory.mem).
+  Determinism.world -> list Values.val -> Memimpl.Mem.mem ->
+  option (Determinism.world * Events.trace * Values.val * Memimpl.Mem.mem).
 
 Axiom do_external_function_possible_trace:
   forall id sg ge w vargs m w' t vres m',
@@ -33,9 +38,7 @@ Axiom do_external_function_possible_trace:
 (** Then, we use this axiomatization to instantiate the actual
     semantics of external functions. *)
 
-Check Events.external_functions_sem.
-
-Definition external_functions_sem :
+Definition external_functions_sem:
   String.string -> AST.signature -> Events.extcall_sem :=
   fun id sg ge vargs m t vres m' =>
     exists w w',
@@ -44,8 +47,8 @@ Definition external_functions_sem :
 Lemma do_external_function_sound:
    forall (id : String.string) (sg : AST.signature) 
      (ge0 : Globalenvs.Senv.t) (vargs : list Values.val)
-     (m : Memory.mem) (t : Events.trace) (vres : Values.val)
-     (m' : Memory.mem) (w w' : Determinism.world),
+     (m : Memimpl.Mem.mem) (t : Events.trace) (vres : Values.val)
+     (m' : Memimpl.Mem.mem) (w w' : Determinism.world),
    do_external_function id sg ge0 w vargs m = Some (w', t, vres, m') ->
    external_functions_sem id sg ge0 vargs m t vres m' /\
    Determinism.possible_trace w t w'.
@@ -59,8 +62,8 @@ Qed.
 Lemma do_external_function_complete:
    forall (id : String.string) (sg : AST.signature) 
      (ge0 : Globalenvs.Senv.t) (vargs : list Values.val)
-     (m : Memory.mem) (t : Events.trace) (vres : Values.val)
-     (m' : Memory.mem) (w w' : Determinism.world),
+     (m : Memimpl.Mem.mem) (t : Events.trace) (vres : Values.val)
+     (m' : Memimpl.Mem.mem) (w w' : Determinism.world),
    external_functions_sem id sg ge0 vargs m t vres m' ->
    Determinism.possible_trace w t w' ->
    do_external_function id sg ge0 w vargs m = Some (w', t, vres, m').
@@ -70,6 +73,9 @@ Proof.
   eapply do_external_function_possible_trace; eauto.
 Qed.
 
+Local Existing Instance Events.symbols_inject_instance.
+Existing Instance StackADT.inject_perm_all.
+
 Axiom external_functions_properties:
   forall id sg, Events.extcall_properties (external_functions_sem id sg) sg.
 
@@ -78,8 +84,8 @@ Axiom external_functions_properties:
 
 Definition do_inline_assembly:
   String.string -> AST.signature -> Globalenvs.Senv.t ->
-  Determinism.world -> list Values.val -> Memory.mem ->
-  option (Determinism.world * Events.trace * Values.val * Memory.mem)
+  Determinism.world -> list Values.val -> Memimpl.Mem.mem ->
+  option (Determinism.world * Events.trace * Values.val * Memimpl.Mem.mem)
   :=
     fun _ _ _ _ _ _ => None.
 
@@ -100,8 +106,8 @@ Qed.
 Lemma do_inline_assembly_sound:
    forall (txt : String.string) (sg : AST.signature)
      (ge0 : Globalenvs.Senv.t) (vargs : list Values.val)
-     (m : Memory.mem) (t : Events.trace) (vres : Values.val)
-     (m' : Memory.mem) (w w' : Determinism.world),
+     (m : Memimpl.Mem.mem) (t : Events.trace) (vres : Values.val)
+     (m' : Memimpl.Mem.mem) (w w' : Determinism.world),
    do_inline_assembly txt sg ge0 w vargs m = Some (w', t, vres, m') ->
    inline_assembly_sem txt sg ge0 vargs m t vres m' /\
    Determinism.possible_trace w t w'.
@@ -112,8 +118,8 @@ Qed.
 Lemma do_inline_assembly_complete:
  forall (txt : String.string) (sg : AST.signature) 
    (ge0 : Globalenvs.Senv.t) (vargs : list Values.val) 
-   (m : Memory.mem) (t : Events.trace) (vres : Values.val)
-   (m' : Memory.mem) (w w' : Determinism.world),
+   (m : Memimpl.Mem.mem) (t : Events.trace) (vres : Values.val)
+   (m' : Memimpl.Mem.mem) (w w' : Determinism.world),
    inline_assembly_sem txt sg ge0 vargs m t vres m' ->
    Determinism.possible_trace w t w' ->
    do_inline_assembly txt sg ge0 w vargs m = Some (w', t, vres, m').
@@ -121,15 +127,42 @@ Proof.
   intros; edestruct inline_assembly_sem_empty; eauto.
 Qed.
 
+Local Instance external_calls_ops: Events.ExternalCallsOps Memimpl.Mem.mem.
+Proof.
+  split.
+  + apply external_functions_sem.
+  + apply external_functions_sem.
+  + apply external_functions_sem.
+  + apply inline_assembly_sem.
+Defined.
+
+Local Instance external_calls_prf: Events.ExternalCallsProps Memimpl.Mem.mem.
+Proof.
+  constructor.
+  + apply external_functions_properties.
+  + apply external_functions_properties.
+  + apply external_functions_properties.
+  + split; intros; edestruct inline_assembly_sem_empty; eauto.
+Qed.
+
+Local Instance enable_builtins_instance: !Events.EnableBuiltins Memimpl.Mem.mem.
+Proof.
+  constructor.
+  exact true.
+Qed.
+
+Local Instance external_calls_instance: Events.ExternalCalls Memimpl.Mem.mem.
+
+
 (** ** Instantiate Cexec. *)
 
 (** Force [Cexec] to be extracted with the memory model instantiated. *)
 
 Definition state := Csem.state.
-Definition do_step ge := Cexec.do_step ge do_external_function do_inline_assembly.
+Definition do_step ge := Cexec.do_step ge do_external_function do_external_function do_external_function do_inline_assembly.
 Definition do_initial_state := Cexec.do_initial_state.
 Definition at_final_state := Cexec.at_final_state.
-Definition step_expr ge := Cexec.step_expr ge do_external_function do_inline_assembly.
+Definition step_expr ge := Cexec.step_expr ge do_external_function do_external_function do_external_function do_inline_assembly.
 (* the following is needed because Mem.MemoryModelOps is after F, V. *)
 Definition init_mem F V := Globalenvs.Genv.init_mem (F := F) (V := V).
 Arguments init_mem [_ _] _.
@@ -139,9 +172,7 @@ Theorem do_step_sound fsr ge:
   List.In (Cexec.TR rule t S') (do_step ge fsr w S) ->
   Csem.step fsr ge S t S' \/ (t = Events.E0 /\ S' = Csem.Stuckstate /\ Cexec.can_crash_world ge fsr w S).
 Proof.
-  apply Cexec.do_step_sound; intros.
-  Check do_external_function_sound.
-  apply (do_external_function_sound _ _ _ _ _ _ _ _ _ _ H).
+  apply Cexec.do_step_sound;
   eauto using
     do_external_function_sound, do_external_function_complete,
     do_inline_assembly_sound, do_inline_assembly_complete.
