cfrontend/SimplExpr_old.v
@@ -17,13 +17,13 @@ Require Import Coqlib.
 Require Import Errors.
 Require Import Integers.
 Require Import Floats.
-Require Import Values.
-Require Import Memory.
-Require Import AST.
-Require Import Ctypes.
-Require Import Cop.
-Require Import Csyntax.
-Require Import Clight.
+Require Import Values_old.
+Require Import Memory_old.
+Require Import AST_old.
+Require Import Ctypes_old.
+Require Import Cop_old.
+Require Import Csyntax_old.
+Require Import Clight_old.
 
 Local Open Scope string_scope.
 
@@ -97,6 +97,11 @@ Definition makeseq (l: list statement) : statement :=
 
 (** Smart constructor for [if ... then ... else]. *)
 
+(** NOTE: Here, we no longer need anything about the memory model,
+    by replacing (Mem.valid_block Mem.empty) with (fun _ => false).
+    See the Cop.SemCast class, and the sem_cast_unit instance.
+ *)
+
 Fixpoint eval_simpl_expr (a: expr) : option val :=
   match a with
   | Econst_int n _ => Some(Vint n)
@@ -106,7 +111,7 @@ Fixpoint eval_simpl_expr (a: expr) : option val :=
   | Ecast b ty =>
       match eval_simpl_expr b with
       | None => None
-      | Some v => sem_cast v (typeof b) ty Mem.empty
+      | Some v => sem_cast v (typeof b) ty tt
       end
   | _ => None
   end.
@@ -114,7 +119,7 @@ Fixpoint eval_simpl_expr (a: expr) : option val :=
 Function makeif (a: expr) (s1 s2: statement) : statement :=
   match eval_simpl_expr a with
   | Some v =>
-      match bool_val v (typeof a) Mem.empty with
+      match bool_val v (typeof a) tt with
       | Some b => if b then s1 else s2
       | None   => Sifthenelse a s1 s2
       end
